\documentclass{article}

\input{vars.tex}
\input{common.tex}

\usepackage{blindtext}
\usepackage[a4paper, total={6in, 8in}]{geometry}

\makeatletter
\newcommand{\defeq}{\vcentcolon=}
\newcommand{\@giventhatstar}[2]{\left(#1\;\middle|\;#2\right)}
\newcommand{\@giventhatnostar}[3][]{#1(#2\;#1|\;#3#1)}
\newcommand{\giventhat}{\@ifstar\@giventhatstar\@giventhatnostar}
\newcommand\problike[2]{\def\probname{#1}\def\probp1{#2}\problikeaux}
\newcommand\problikeaux[1][]{%
  \ifx\relax#1\relax%
    \probname(\probp1)
  \else%
    \probname\giventhat{\probp1}{#1}
  \fi
}
\newcommand\prob{\problike{Pr}}
\newcommand\pre{\problike{H}}
\newcommand\pri{\problike{I}}
\newcommand\prt[2]{\problike{P}{#1 \rightarrow #2}}
\newcommand\prtf[3]{\problike{P_{#1}}{#2 \rightarrow #3}}
\DeclareRobustCommand\iff{\;\Longleftrightarrow\;}
\makeatother

\newcommand\bigforall{%
  \mathop{\lower0.75ex\hbox{\ensuremath{%
    \mathlarger{\mathlarger{\mathlarger{\mathlarger{\forall}}}}}}}%
  \limits}

\newcommand\bigexists{%
  \mathop{\lower0.75ex\hbox{\ensuremath{%
    \mathlarger{\mathlarger{\mathlarger{\mathlarger{\exists}}}}}}}%
  \limits}

\title{Teoria informacji kolokwium 4 grudnia 2024}

\begin{document}

\maketitle

\section{Problem 2}

\subsection{Task 1}

We observe that for binary input and perfect channel combined in series with Z-channel we have:
\begin{equation}
\begin{cases}
    \prtf{A}{\alpha}{\alpha} = 1 \\
    \prtf{A}{\beta}{\beta} = 1 \\
    \prtf{B}{\alpha}{\alpha} = 1-p \\
    \prtf{B}{\alpha}{\beta} = p \\
    \prtf{B}{\beta}{\beta} = 1
\end{cases}
\end{equation}

$\prob{B}[A,C]$ won't be well defined for a channel matrix, because:
\begin{equation}
\begin{cases}
\prob{B=\alpha}[A=\alpha, C=\beta] = 1 \\
\prob{B=\alpha}[A=\alpha, C=\alpha] = 1
\end{cases}
\end{equation}

Hence the requirement that there are no zero elements in matrices of both channels will come into play.
We consider the probability to be well defined if:

\begin{enumerate}
\item $\bigexists_{f \perp P(A)}{\bigforall_{\substack{a \in A \\ c \in C}}{ \prob{B=b}[A=a, C=c] = f(...) }}$
\item $\bigforall_{\substack{a \in A \\ c \in C}}{ 0 < \prob{B=b}[A=a, C=c] < 1 }$
\item $\bigforall_{\substack{a \in A \\ c \in C}}{ \sum_{b \in B}{\prob{B=b}[A=a, C=c]} = 1 }$
\end{enumerate}

Now let's start by expanding the probability using Bayes' theorem:
\begin{equation}
\prob{b}[a,c] = \frac{ \prob{a,c}[b]*\prob{b} }{ \prob{a,c} }
\end{equation}

For numerator we use the fact that $\prob{x,y}[z] = \prob{x}[y,z]*\prob{y}[z]$ and for enumerator we use $\prob{x,y}=\prob{x}[y]*\prob{y}$:
\begin{equation}
\prob{b}[a,c] = \frac{ \prob{a}[b,c]*\prob{b}*\prob{c}[b] }{ \prob{a}[c] * \prob{c} }
\end{equation}

Now we use conditional independence contraint so $\prob{a}[b,c] = \prob{a}[b]$:
\begin{equation}
\prob{b}[a,c] = \frac{ \prob{a}[b]*\prob{b}*\prob{c}[b] }{ \prob{a}[c] * \prob{c} }
\end{equation}

We use the fact that $\prob{x}[y] = \prob{y}[x] * \frac{\prob{x}}{\prob{y}}$:
\begin{equation}
\prob{b}[a,c] = \frac{ \prob{b}[a]*\prob{a}*\prob{b}*\prob{c}[b] }{ \prob{a}[c] * \prob{c} * \prob{b} }
\end{equation}

After reorganising terms:
\begin{equation}
\prob{b}[a,c] = (\prob{b}[a] * \prob{c}[b]) * \frac{ \prob{a} }{ \prob{a}[c] } * \frac{1}{\prob{c}}
\end{equation}

Now let's observe that $\frac{\prob{x}}{\prob{x}[y]} = \frac{\prob{y}}{\prob{y}[x]}$:
\begin{equation}
\prob{b}[a,c] = (\prob{b}[a] * \prob{c}[b]) * \frac{ \prob{c} }{ \prob{c}[a] } * \frac{1}{\prob{c}}
\end{equation}

This can be written as:
\begin{equation}
\prob{b}[a,c] = \prtf{\Gamma_1}{a}{b} * \prtf{\Gamma_2}{b}{c} * \frac{ 1 }{ \prob{c}[a] }
\end{equation}

We observe that $\prob{c}[a]$ in fact does not depend on the distribution of $A$, which proves first point.
In all our transformations we inmplicitly use the facts that $\prob{a}, \prob{b}, \prob{c} \neq 0$
Second point is trivial to show, because $0 < \prtf{\Gamma_1}{a}{b}, \prtf{\Gamma_2}{b}{c}, \prob{c}[a] < 1$
Third point is direct consequence of conditional independence.

\subsection{Task 2}

Let's assume we take channel $\Gamma_E$ and squeeze the symbol space using mapping $s_1 \in {(A \times C)}^{A} \defeq s_1(a,c) = a$

In such scenario:
\begin{gather*}
\prtf{\Gamma_E}{s_1(a,c)}{b} = \sum_{c}{ \prtf{\Gamma_E}{a,c}{b} } \\
\sum_{c}{ \prtf{\Gamma_1}{a}{b} * \prtf{\Gamma_2}{b}{c} * \frac{ 1 }{ \prob{c}[a] } } \\
\prtf{\Gamma_F}{a}{b} = \prtf{\Gamma_1}{a}{b}  * \sum_{c}{ \frac{ \prtf{\Gamma_2}{b}{c} }{ \prob{c}[a] } } 
%(\Gamma_E)_{s_1(a,b), c} = \frac{ 1 }{ \prob{c}[a] } * (\Gamma_1 \times \Gamma_2)_{a,c}
\end{gather*}

We know that $\sum_{c}{\prob{c}[a]} = 1$

If we compare $\prtf{\Gamma_F}{a}{b}$ and $\prtf{\Gamma_1}{a}{b}$ then in $I(A,B)$ we will notice that in worst case we can select such a coefficients that $\Gamma_F$ is as bad as using $\Gamma_1$
The original matrix $\Gamma_F$ has more rows than $\Gamma_E$ (such that rows of $\Gamma_F$ are linear combinations of $\Gamma_E$) meaning that the capacity of original $Gamma_E$ cannot be lower.

Hance we prove that capacity of $\Gamma_E$ is no lower than $\Gamma_F$

\subsection{Task 3}

My best guess is that we use some prime factors to make $\Gamma_E$ have all rows independent, then that will work. However I was unable to showcase some concrete example.

\end{document}
