\documentclass{article}

\input{vars.tex}
\input{common.tex}

\usepackage{blindtext}
\usepackage[a4paper, total={6in, 8in}]{geometry}

\makeatletter
\newcommand{\defeq}{\vcentcolon=}
\newcommand{\@giventhatstar}[2]{\left(#1\;\middle|\;#2\right)}
\newcommand{\@giventhatnostar}[3][]{#1(#2\;#1|\;#3#1)}
\newcommand{\giventhat}{\@ifstar\@giventhatstar\@giventhatnostar}
\newcommand\problike[2]{\def\probname{#1}\def\probp1{#2}\problikeaux}
\newcommand\problikeaux[1][]{%
  \ifx\relax#1\relax%
    \probname(\probp1)
  \else%
    \probname\giventhat{\probp1}{#1}
  \fi
}
\newcommand\prob{\problike{Pr}}
\newcommand\pre{\problike{H}}
\newcommand\pri{\problike{I}}
\makeatother

\newcommand\bigexists{%
  \mathop{\lower0.75ex\hbox{\ensuremath{%
    \mathlarger{\mathlarger{\mathlarger{\mathlarger{\exists}}}}}}}%
  \limits}

\title{Teoria informacji kolokwium 4 grudnia 2024}

\begin{document}

\maketitle

\section{Problem 3}

%$\prob{Y=y}[X=x] = \prob{F(x)=y}[X=x] = \prob{F(x) = y} = 1/n$
%$\pri{Y,F} = \pre{Y} - \pre{Y}[F] = \log_2{n} -  $

I we use the "triangle" inequality i.e $\pre{C}[B] + \pre{B}[A] \geq \pre{C}[A]$ for:
\begin{equation}
\begin{cases}
    A=Y\\
    B=g(Y)\\
    C=f(X)
\end{cases}
\mbox{and}
\begin{cases}
    A=X\\
    B=f(X)\\
    C=g(Y)
\end{cases}
\end{equation}
We get:
\begin{equation}
\begin{cases}
    \pre{f(X)}[g(Y)] + \pre{g(Y)}[Y] \geq \pre{f(X)}[Y] \\
    \pre{g(Y)}[f(X)] + \pre{f(X)}[X] \geq \pre{g(Y)}[X]
\end{cases}
\implies
\begin{cases}
    \pre{f(X)}[g(Y)] + 0 \geq \pre{f(X)}[Y] \\
    \pre{g(Y)}[f(X)] + 0 \geq \pre{g(Y)}[X]
\end{cases}
\end{equation}

If we add those equalities side-by-side and move to the right, we get:
\begin{align*}
0 \geq - \pre{f(X)}[g(Y)] - \pre{g(Y)}[f(X)] + \pre{f(X)}[Y] + \pre{g(Y)}[X]
\end{align*}

Let's consider $X=Y$ it can be alternativelly expressed as:
\begin{gather*}
\pre{f(X)}[g(X)] + \pre{g(X)}[f(X)] \geq 0 \\
\pre{f(X),g(X)}-\pri{f(X);g(X)} \geq 0 \\
\pre{f(X),g(X)} \geq \pri{f(X);g(X)}
\end{gather*}

Now with that if we look at this equation we can observe that for:
\begin{enumerate}
    \item $f = g = id$: the equality happen
    \item $f, g \defeq const$: the equality happen and every term is zeroed
    \item $X = Y, f = g$: the equality happen
    \item $X \perp Y$: the equality happen
\end{enumerate}

Looking at those observations (and first of the equations) we can conclude that condition implying strict inequality is as follows:
\begin{equation}
\bigexists_{\substack{x, x' \in X \\ y, y' \in Y \\ \prob{X=x \land Y=y} > 0}}{\prob{X=x \land Y=y} \neq \prob{X=x}*\prob{Y=y} \land g(x) = g(x') \land f(y) \neq f(y')}
\end{equation}

Now to prove the inequality in the exercice, we add and substract joint entropy of $f(X)$ and $g(Y)$:
\begin{equation}
0 \geq \pre{f(X), g(Y)} - \pre{f(X)}[g(Y)] - \pre{g(Y)}[f(X)] + (\pre{f(X)}[Y] + \pre{g(Y)}[X] - \pre{f(X), g(Y)})
\end{equation}

We now use the fact that we can "extend" entropy to joint entropy for functions: $\pre{f(X)}[Y] = \pre{f(X),g(Y)}[Y]$ (analogical for $\pre{g(Y)}[X]$):
\begin{gather*}
0 \geq (\pre{f(X), g(Y)} - \pre{f(X)}[g(Y)] - \pre{g(Y)}[f(X)]) + \\
    (\pre{f(X),g(Y)}[Y] + \pre{f(X),g(Y)}[X] - \pre{f(X), g(Y)})
\end{gather*}

Adding empty term $\pre{f(X),g(Y)}[X,Y]$:
\begin{gather*}
0 \geq (\pre{f(X), g(Y)} - \pre{f(X)}[g(Y)] - \pre{g(Y)}[f(X)]) + \\
(-\pre{f(X),g(Y)}[X,Y] + \pre{f(X),g(Y)}[Y] + \pre{f(X),g(Y)}[X] - \pre{f(X), g(Y)})
\end{gather*}

Now we use the fact that $\pri{A; B} = \pre{A,B} - \pre{A}[B] - \pre{B}[A]$
\begin{equation}
0 \geq \pri{f(X); g(Y)} + (- \pre{f(X),g(Y)}[X,Y] + \pre{f(X),g(Y)}[Y] + \pre{f(X),g(Y)}[X] - \pre{f(X), g(Y)})
\end{equation}

We add $\pri{X;Y}$ on both sides:
\begin{gather*}
\pri{X;Y} \geq \pri{f(X); g(Y)} + \\
(\pri{X;Y} - \pre{f(X),g(Y)}[X,Y] + \pre{f(X),g(Y)}[X] + \pre{f(X),g(Y)}[Y] - \pre{f(X), g(Y)})
\end{gather*}

We assume $Z \defeq f(X),g(Y)$ and look at the terms in bracket:
\begin{equation}
\pri{X;Y} - \pre{Z}[X,Y] + \pre{Z}[X] + \pre{Z}[Y] - \pre{Z}
\end{equation}

We expand by definition of mutual information and use
the "condition inversion rule"

Rule: $\pre{Y}[X] = \pre{X}[Y] + \pre{Y} - \pre{X}$


\begin{align*}
(\pre{X} + \pre{Y} - \pre{X,Y}) \\
- (\pre{X,Y}[Z] + \pre{Z} - \pre{X,Y}) \\
+ (\pre{X}[Z] + \pre{Z} - \pre{X}) \\
+ (\pre{Y}[Z] + \pre{Z} - \pre{Y}) - \pre{Z}
\end{align*}

After adding everything up:
\begin{equation}
-\pre{X,Y}[Z] + \pre{X}[Z] + \pre{Y}[Z]
\end{equation}

Which is just a mutual information:
\begin{equation}
-\pre{X,Y}[Z] + \pre{X}[Z] + \pre{Y}[Z] = \pri{X;Y}[Z]
\end{equation}


If we summarize that we get desired relation:
\begin{equation}
\pri{X;Y} \geq \pri{f(X); g(Y)} + \pri{X;Y}[f(X), g(Y)]
\end{equation}

As a side note (as I often used it and I'm not entirely sure if that is considered "basic" enough, so provide quick side-note for completeness sake) we can deliver "triangle" inequality from:
\begin{equation}
\pre{Y}[X] + \pre{Z}[Y] \geq \pre{Y}[X] + \pre{Z}[Y,X] = \pre{Y,Z}[X] \geq \pre{Z}[X]
\end{equation}

\end{document}
